Constant-time buffer comparison and remove all remaining assume/lax from lib

lib/fst/Lib.ByteBuffer.fst
@@ -5,14 +5,31 @@ open FStar.HyperStack.ST
 open LowStar.Buffer
 
 open Lib.IntTypes
-open Lib.RawIntTypes
 open Lib.Buffer
 
 module ST = FStar.HyperStack.ST
-
 module Loops = Lib.LoopCombinators
+module Raw = Lib.RawIntTypes
 
 friend Lib.ByteSequence
+friend Lib.IntTypes
+
+(*
+ * Despite befriending IntTypes this module enforces secrecy.
+ *
+ * We befriend IntTypes (or use RawIntTypes) to call into KreMLin C library 
+ * for endianness conversions, which uses public machine integers.
+ * E.g. `uint_to_bytes_le` loads a secret integer into a buffer of secret bytes by
+ * internally casting the integer to a public machine integer, calling into KreMLin,
+ * and converting the result back to secret bytes.
+ *
+ * We use RawIntTypes when possible and only when this would be inconvenient
+ * rely on opening the definitions in IntTypes. Specifically, only
+ * `uint_from_bytes_le`, uint_from_bytes_be`, `uint_to_bytes_le`, and `uint_to_bytes_be` 
+ * rely on definitions in IntTypes. Alternatively, RawIntTypes could be used to cast 
+ * sequences and buffers of secret integers to sequences and buffers of machine integers,
+ * but this would be too cumbersome.
+*)
 
 #set-options "--z3rlimit 50 --max_fuel 0 --max_ifuel 1"
 
@@ -20,127 +37,90 @@ let uint_to_be #t #l u =
   match t, l with
   | U1, _ -> u
   | U8, _ -> u
-  | U16, SEC -> 
-    RawIntTypes.u16_from_UInt16 (C.Endianness.htobe16 (RawIntTypes.u16_to_UInt16 u))
   | U16, PUB -> C.Endianness.htobe16 u
-  | U32, SEC -> C.Endianness.htobe32 u
-  | U64,_ -> C.Endianness.htobe64 u
+  | U16, SEC -> Raw.u16_from_UInt16 (C.Endianness.htobe16 (Raw.u16_to_UInt16 u))
+  | U32, PUB -> C.Endianness.htobe32 u
+  | U32, SEC -> Raw.u32_from_UInt32 (C.Endianness.htobe32 (Raw.u32_to_UInt32 u))
+  | U64, PUB -> C.Endianness.htobe64 u
+  | U64, SEC -> Raw.u64_from_UInt64 (C.Endianness.htobe64 (Raw.u64_to_UInt64 u))
 
 let uint_to_le #t #l u =
-  match t with
-  | U1 -> u
-  | U8 -> u
-  | U16 -> C.Endianness.htole16 u
-  | U32 -> C.Endianness.htole32 u
-  | U64 -> C.Endianness.htole64 u
+  match t, l with
+  | U1, _ -> u
+  | U8, _ -> u
+  | U16, PUB -> C.Endianness.htole16 u
+  | U16, SEC -> Raw.u16_from_UInt16 (C.Endianness.htole16 (Raw.u16_to_UInt16 u))
+  | U32, PUB -> C.Endianness.htole32 u
+  | U32, SEC -> Raw.u32_from_UInt32 (C.Endianness.htole32 (Raw.u32_to_UInt32 u))
+  | U64, PUB -> C.Endianness.htole64 u
+  | U64, SEC -> Raw.u64_from_UInt64 (C.Endianness.htole64 (Raw.u64_to_UInt64 u))
 
 let uint_from_be #t #l u =
-  match t with
-  | U1 -> u
-  | U8 -> u
-  | U16 -> C.Endianness.be16toh u
-  | U32 -> C.Endianness.be32toh u
-  | U64 -> C.Endianness.be64toh u
+  match t, l with
+  | U1, _ -> u
+  | U8, _ -> u
+  | U16, PUB -> C.Endianness.be16toh u
+  | U16, SEC -> Raw.u16_from_UInt16 (C.Endianness.be16toh (Raw.u16_to_UInt16 u))
+  | U32, PUB -> C.Endianness.be32toh u
+  | U32, SEC -> Raw.u32_from_UInt32 (C.Endianness.be32toh (Raw.u32_to_UInt32 u))
+  | U64, PUB -> C.Endianness.be64toh u
+  | U64, SEC -> Raw.u64_from_UInt64 (C.Endianness.be64toh (Raw.u64_to_UInt64 u))
 
 let uint_from_le #t #l u =
-  match t with
-  | U1 -> u
-  | U8 -> u
-  | U16 -> C.Endianness.le16toh u
-  | U32 -> C.Endianness.le32toh u
-  | U64 -> C.Endianness.le64toh u
+  match t, l with
+  | U1, _ -> u
+  | U8, _ -> u
+  | U16, PUB -> C.Endianness.le16toh u
+  | U16, SEC -> Raw.u16_from_UInt16 (C.Endianness.le16toh (Raw.u16_to_UInt16 u))
+  | U32, PUB -> C.Endianness.le32toh u
+  | U32, SEC -> Raw.u32_from_UInt32 (C.Endianness.le32toh (Raw.u32_to_UInt32 u))
+  | U64, PUB -> C.Endianness.le64toh u
+  | U64, SEC -> Raw.u64_from_UInt64 (C.Endianness.le64toh (Raw.u64_to_UInt64 u))
 
-/// BEGIN Constant-time buffer equality
-
-inline_for_extraction noextract
-val cmp_bytes: 
-    #len1:size_t 
-  -> #len2:size_t 
-  -> b1:lbuffer uint8 len1 
-  -> b2:lbuffer uint8 len2 
-  -> len:size_t{v len <= v len1 /\ v len <= v len2} 
-  -> res:lbuffer uint8 (size 1) ->
-  Stack uint8
-    (requires fun h -> 
-      live h b1 /\ live h b2 /\ live h res /\ disjoint res b1 /\ disjoint res b2 /\
-      v (bget h res 0) == 255)    
-    (ensures fun h0 z h1 -> 
-      modifies1 res h0 h1 /\
-      (as_seq h0 (gsub b1 0ul len) == as_seq h0 (gsub b2 0ul len)  ==> v z == 255) /\
-      (as_seq h0 (gsub b1 0ul len) =!= as_seq h0 (gsub b2 0ul len) ==> v z == 0))
-let rec cmp_bytes #len1 #len2 b1 b2 len res =
-  let a_spec i = uint8 in
-  let refl h = bget h res 0 in
-  let footprint i = loc res in
-  let spec h = 
-  let h0 = ST.get() in
-  loop h0 len a_spec refl footprint
-    (fun i ->
-      Loops.unfold_repeat_gen len a_spec (spec h0) (refl h0 0);
-      let z0 = res.(0ul) in
-      res.(0ul) <- eq_mask b1.(i) b2.(i) &. z0
-    )
-
-
-(*
-  UInt.logand_lemma_1 #8 255;
-  UInt.logand_lemma_2 #8 255;
-  UInt.logand_lemma_1 #8 0;
-  UInt.logand_lemma_2 #8 0;
+let rec eq_mask #t #len1 #len2 b1 b2 len res =
   let h0 = ST.get() in
   let inv h (i:nat{i <= v len}) =
-    let z = bget h res 0 in
     modifies1 res h0 h /\
-    (as_seq h0 (gsub b1 0ul (size i)) == as_seq h0 (gsub b2 0ul (size i))  ==> v z == 255) /\
-    (as_seq h0 (gsub b1 0ul (size i)) =!= as_seq h0 (gsub b2 0ul (size i)) ==> v z == 0)
+    v (bget h res 0) == v (BS.eq_mask (as_seq h0 b1) (as_seq h0 b2) i)
   in
-  Loops.for 0ul len inv 
+  Lib.Loops.for 0ul len inv
     (fun i ->
       let z0 = res.(0ul) in
-      res.(0ul) <- eq_mask b1.(i) b2.(i) &. z0;
-      let h = ST.get() in
-      if v (bget h res 0) = 255 then
-        begin
-        let s1 = as_seq h0 (gsub b1 0ul (i +! 1ul)) in
-        let s2 = as_seq h0 (gsub b2 0ul (i +! 1ul)) in
-        FStar.Seq.lemma_split s1 (v i);
-        FStar.Seq.lemma_split s2 (v i);       
-        Seq.lemma_eq_intro s1 s2
-        end
-      else if v z0 = 0 then
-        lemma_not_equal_slice (as_seq h0 b1) (as_seq h0 b2) 0 (v i) (v i + 1)
-      else
-        lemma_not_equal_last (as_seq h0 b1) (as_seq h0 b2) 0 (v i + 1));
+      res.(0ul) <- IntTypes.eq_mask b1.(i) b2.(i) &. res.(0ul);
+      let z = res.(0ul) in
+      assert (z == BS.eq_mask_inner (as_seq h0 b1) (as_seq h0 b2) (v len) (v i) z0));
   res.(0ul)
 
 let lbytes_eq #len b1 b2 =
   push_frame();
   let res = create 1ul (u8 255) in
-  let z = cmp_bytes b1 b2 len res in
+  let z = eq_mask b1 b2 len res in
   pop_frame();
-  z = u8 255
+  Raw.u8_to_UInt8 z = 255uy
 
-/// END Constant-time buffer equality
+#set-options "--max_fuel 1 --max_ifuel 1"
 
-#set-options "--initial_fuel 1 --max_fuel 1 --max_ifuel 1"
+/// BEGIN using friend Lib.IntTypes
 
-val foo: l:secrecy_level -> b:Seq.seq UInt8.t ->
-  Lemma (ensures (BS.nat_from_bytes_le #l b == Kremlin.Endianness.le_to_n b)) 
+val nat_from_bytes_le_to_n: l:secrecy_level -> b:Seq.seq UInt8.t ->
+  Lemma (ensures (BS.nat_from_bytes_le #l b == Kremlin.Endianness.le_to_n b))
   (decreases (Seq.length b))
-let rec foo l b = 
-  if Seq.length b = 0 then () else foo l (Seq.tail b)
+let rec nat_from_bytes_le_to_n l b =
+  if Seq.length b = 0 then ()
+  else nat_from_bytes_le_to_n l (Seq.tail b)
 
-val bar: l:secrecy_level -> b:Seq.seq UInt8.t ->
-  Lemma (ensures (BS.nat_from_bytes_be #l b == Kremlin.Endianness.be_to_n b)) 
+val nat_from_bytes_be_to_n: l:secrecy_level -> b:Seq.seq UInt8.t ->
+  Lemma (ensures (BS.nat_from_bytes_be #l b == Kremlin.Endianness.be_to_n b))
   (decreases (Seq.length b))
-let rec bar l b = 
-  if Seq.length b = 0 then () else bar l (Seq.slice b 0 (Seq.length b - 1))
+let rec nat_from_bytes_be_to_n l b =
+  if Seq.length b = 0 then ()
+  else nat_from_bytes_be_to_n l (Seq.slice b 0 (Seq.length b - 1))
 
 let uint_from_bytes_le #t #l i =
   let h0 = ST.get () in
-  foo l (as_seq h0 i);
+  nat_from_bytes_le_to_n l (as_seq h0 i);
   match t with
-  | U8 -> i.(0ul) 
+  | U8 -> i.(0ul)
   | U16 -> let u = C.load16_le i in cast #t #l U16 l u
   | U32 -> let u = C.load32_le i in cast #t #l U32 l u
   | U64 -> let u = C.load64_le i in cast #t #l U64 l u
@@ -148,7 +128,7 @@ let uint_from_bytes_le #t #l i =
 
 let uint_from_bytes_be #t #l i =
   let h0 = ST.get () in
-  bar l (as_seq h0 i);
+  nat_from_bytes_be_to_n l (as_seq h0 i);
   match t with
   | U8 -> i.(0ul)
   | U16 -> let u = C.load16_be i in cast #t #l U16 l u
@@ -156,152 +136,128 @@ let uint_from_bytes_be #t #l i =
   | U64 -> let u = C.load64_be i in cast #t #l U64 l u
   | U128 -> let u = C.load128_be i in cast #t #l U128 l u
 
-let uint_to_bytes_le #t #l o i = 
+val nat_to_bytes_n_to_le: len:size_nat -> l:secrecy_level -> n:nat{n < pow2 (8 * len)} ->
+  Lemma (ensures (Seq.equal (Kremlin.Endianness.n_to_le (size len) n)
+                            (BS.nat_to_bytes_le #l len n)))
+  (decreases len)
+let rec nat_to_bytes_n_to_le len l n =
+  if len = 0 then () else
+    begin
+    Math.Lemmas.division_multiplication_lemma n (pow2 8) (pow2 (8 * (len - 1)));
+    Math.Lemmas.pow2_plus 8 (8 * (len - 1));
+    nat_to_bytes_n_to_le (len - 1) l (n / 256)
+    end
+
+val nat_to_bytes_n_to_be: len:size_nat -> l:secrecy_level -> n:nat{n < pow2 (8 * len)} ->
+  Lemma (ensures (Seq.equal (Kremlin.Endianness.n_to_be (size len) n)
+                            (BS.nat_to_bytes_be #l len n)))
+  (decreases len)
+let rec nat_to_bytes_n_to_be len l n =
+  if len = 0 then () else
+    begin
+    Math.Lemmas.division_multiplication_lemma n (pow2 8) (pow2 (8 * (len - 1)));
+    Math.Lemmas.pow2_plus 8 (8 * (len - 1));
+    nat_to_bytes_n_to_be (len - 1) l (n / 256)
+    end
+
+let uint_to_bytes_le #t #l o i =
   match t with
-  | U8 -> o.(0ul) <- i
-  | _ -> admit() 
-  | U16 -> C.store16_le o (u16_to_UInt16 i)
-  | U32 -> C.store32_le o (u32_to_UInt32 i)
-  | U64 -> C.store64_le o (u64_to_UInt64 i)
-  | U128 -> C.store128_le o (u128_to_UInt128 i)
+  | U1 | U8 ->
+    o.(0ul) <- i;
+    let h1 = ST.get () in
+    assert (Seq.equal (as_seq h1 o) (BS.nat_to_bytes_le_ #l (numbytes t) (Raw.uint_to_nat i)))
+  | U16 ->
+    C.store16_le o (Raw.u16_to_UInt16 i);
+    let h1 = ST.get () in
+    nat_to_bytes_n_to_le (numbytes t) l (v i)
+  | U32 ->
+    C.store32_le o (Raw.u32_to_UInt32 i);
+    let h1 = ST.get () in
+    nat_to_bytes_n_to_le (numbytes t) l (v i)
+  | U64 ->
+    C.store64_le o (Raw.u64_to_UInt64 i);
+    let h1 = ST.get () in
+    nat_to_bytes_n_to_le (numbytes t) l (v i)
+  | U128 ->
+    C.store128_le o (Raw.u128_to_UInt128 i);
+    let h1 = ST.get () in
+    nat_to_bytes_n_to_le (numbytes t) l (v i)
 
 let uint_to_bytes_be #t #l o i =
   match t with
-  | U8 -> o.(0ul) <- i
-  | U16 -> C.store16_be o (u16_to_UInt16 i)
-  | U32 -> C.store32_be o (u32_to_UInt32 i)
-  | U64 -> C.store64_be o (u64_to_UInt64 i)
-  | U128 -> C.store128_be o (u128_to_UInt128 i)
+  | U1 | U8 ->
+    o.(0ul) <- i;
+    let h1 = ST.get () in
+    assert (Seq.equal (as_seq h1 o) (BS.nat_to_bytes_be_ #l (numbytes t) (Raw.uint_to_nat i)))
+  | U16 ->
+    C.store16_be o (Raw.u16_to_UInt16 i);
+    let h1 = ST.get () in
+    nat_to_bytes_n_to_be (numbytes t) l (v i)
+  | U32 ->
+    C.store32_be o (Raw.u32_to_UInt32 i);
+    let h1 = ST.get () in
+    nat_to_bytes_n_to_be (numbytes t) l (v i)
+  | U64 ->
+    C.store64_be o (Raw.u64_to_UInt64 i);
+    let h1 = ST.get () in
+    nat_to_bytes_n_to_be (numbytes t) l (v i)
+  | U128 ->
+    C.store128_be o (Raw.u128_to_UInt128 i);
+    let h1 = ST.get () in
+    nat_to_bytes_n_to_be (numbytes t) l (v i)
 
-inline_for_extraction
-val uints_from_bytes_le':
-    #t:inttype{~(t == U1)}
-  -> #l:secrecy_level
-  -> #len:size_t{v len * numbytes t <= max_size_t}
-  -> o:lbuffer (uint_t t l) len
-  -> i:lbuffer (uint_t U8 l) (len *! size (numbytes t)) ->
-  Stack unit
-        (requires fun h0 -> live h0 o /\ live h0 i /\ disjoint o i)
-        (ensures  fun h0 _ h1 -> 
-          modifies1 o h0 h1)
-         // /\ as_seq h1 o == BS.uints_from_bytes_le #t #l #(v len) (as_seq h0 i))
-let uints_from_bytes_le' #t #l #len o i =
-  let h0 = ST.get() in
-  [@ inline_let]
-  let spec h : GTot (j:size_nat{j < v len} -> uint_t t l) =    
-    let i0 = B.as_seq h0 i in
-    fun j ->
-    BS.uint_from_bytes_le (Sequence.sub i0 (j * numbytes t) (numbytes t)) 
-  in
-  let impl (j:size_t{v j < v len}) : Stack (uint_t t l)
-          (requires fun h -> modifies1 (gsub o 0ul j) h0 h)
-          (ensures  fun h r h' -> h == h' /\ r == spec h0 (v j)) 
-  = 
-    let h = ST.get() in
-    let bj = B.sub #(uint_t U8 l) i (mul_mod j (size (numbytes t))) (size (numbytes t)) in
-    let r = uint_from_bytes_le bj in
-//    assume (B.as_seq h bj = 
-    assert (uint_v r == uint_v (BS.uint_from_bytes_le #t #l (B.as_seq h bj)));
-    r
-  in
-  fill #(uint_t t l) h0 len o spec impl
+/// END using friend Lib.IntTypes
 
-(*
-(*
-let uints_from_bytes_le #t #l #len b =
-  let l = create #(uint_t t l) len (nat_to_uint 0) in
-  repeati len
-    (fun i l -> l.[i] <- uint_from_bytes_le (sub b (i * numbytes t) (numbytes t))) l
-*)
+module Seq = Lib.Sequence
 
-inline_for_extraction
 let uints_from_bytes_le #t #l #len o i =
-  assume (l == PUB);
   let h0 = ST.get() in
-  let open Lib.Sequence in
   [@ inline_let]
-  let spec (h0:mem) : GTot (j:size_nat{j < v len} -> lseq (uint_t t l) (v len) ->
-    lseq (uint_t t l) (v len))
-    = 
-    let s0 = as_seq h0 i in
-    fun j s -> s.[j] <- (BS.uint_from_bytes_le (sub s0 (j * numbytes t) (numbytes t)))
+  let spec (h:mem) : GTot (j:size_nat{j < v len} -> uint_t t l) =
+    let i0 = as_seq h i in
+    fun j -> BS.uint_from_bytes_le (Seq.sub i0 (j * numbytes t) (numbytes t))
   in
-  let impl (j:size_t{v j < v len}) : Stack unit
-     (requires loop1_inv h0 len (uint_t t l) len o spec (v j))
-     (ensures  fun _ _ -> loop1_inv h0 len (uint_t t l) len o spec (v j + 1))
-  =
-    let b_i = B.sub #(uint_t U8 l) i (mul_mod j (size (numbytes t))) (size (numbytes t)) in
-    let u_i = uint_from_bytes_le b_i in
-    o.(j) <- u_i; //upd #_ #len o j u_i 
-    let h1 = ST.get() in
-    assume (as_seq h1 o == LoopCombinators.repeati (v j + 1) (spec h0) (as_seq h0 o))
-  in
-  loop1 h0 len o spec impl;
-  let h1 = ST.get() in  
-  assert (loop1_inv h0 len (uint_t t l) len o spec (v len) h1);
-  assume (as_seq h1 o == LoopCombinators.repeati (v len) (spec h0) (as_seq h0 o))
-  
-  admit()
-  
+  fill h0 len o spec (fun j ->
+    let h = ST.get() in
+    let bj = sub i (j *! (size (numbytes t))) (size (numbytes t)) in
+    let r = uint_from_bytes_le bj in
+    as_seq_gsub h i (j *! size (numbytes t)) (size (numbytes t));
+    uintv_extensionality r (spec h0 (v j));
+    r);
+  let h1 = ST.get() in
+  assert (Seq.equal (as_seq h1 o) (BS.uints_from_bytes_le (as_seq h0 i)))
 
-
-  let inv (h1:mem) (j:nat{j <= v len}) = 
-    modifies1 o h0 h1 /\
-    Seq.slice (as_seq h1 o) 0 j == 
-    BS.uints_from_bytes_le #t #l #j (Seq.slice (as_seq h0 i) 0 (j * numbytes t)) 
-  in
-  assert (Seq.slice (as_seq h0 o) 0 0 == Seq.empty);
-  assert (inv h0 0);
-  admit()
-  
-  
-  let f' (j:size_t{0 <= v j /\ v j < v len}) : Stack unit
-      (requires (fun h -> inv h (v j)))
-      (ensures (fun h1 _ h2 -> inv h2 (v j + 1))) =
-      let b_i = sub i (mul_mod j (size (numbytes t))) (size (numbytes t)) in
-      let u_i = uint_from_bytes_le b_i in
-      upd #_ #len o j u_i in
-  Lib.Loops.for 0ul len inv f'
-
-*)
-
-
-inline_for_extraction
 let uints_from_bytes_be #t #l #len o i =
   let h0 = ST.get() in
-  let inv (h1:mem) (j:nat) = live h1 i /\ live h1 o in
-  let f' (j:size_t{0 <= v j /\ v j < v len}) : Stack unit
-      (requires (fun h -> inv h (v j)))
-      (ensures (fun h1 _ h2 -> inv h2 (v j + 1))) =
-      let b_i = sub i (mul_mod j (size (numbytes t))) (size (numbytes t)) in
-      let u_i = uint_from_bytes_be b_i in
-      upd #_ #len o j u_i in
-  admit();
-  Lib.Loops.for 0ul len inv f'
+  [@ inline_let]
+  let spec (h:mem) : GTot (j:size_nat{j < v len} -> uint_t t l) =
+    let i0 = as_seq h i in
+    fun j -> BS.uint_from_bytes_be (Seq.sub i0 (j * numbytes t) (numbytes t))
+  in
+  fill h0 len o spec (fun j ->
+    let h = ST.get() in
+    let bj = sub i (j *! (size (numbytes t))) (size (numbytes t)) in
+    let r = uint_from_bytes_be bj in
+    as_seq_gsub h i (j *! size (numbytes t)) (size (numbytes t));
+    uintv_extensionality r (spec h0 (v j));
+    r);
+  let h1 = ST.get() in
+  assert (Seq.equal (as_seq h1 o) (BS.uints_from_bytes_be (as_seq h0 i)))
 
-inline_for_extraction
 let uints_to_bytes_le #t #l len o i =
   let h0 = ST.get () in
-  let inv (h1:mem) (j:nat) = live h1 i /\ live h1 o in
-  let f' (j:size_t{0 <= v j /\ v j < v len}) : Stack unit
-    (requires (fun h -> inv h (v j)))
-    (ensures  (fun h1 _ h2 -> inv h2 (v j + 1))) =
-      let u_i = i.(j) in
-      let b_i = sub o (mul_mod j (size (numbytes t))) (size (numbytes t)) in
-      uint_to_bytes_le b_i u_i in
-  admit();
-  Lib.Loops.for 0ul len inv f'
+  let a_spec i = unit in
+  let spec (h:mem) = BS.uints_to_bytes_le_inner (as_seq h i) in
+  fill_blocks h0 (size (numbytes t)) len o a_spec (fun _ _ -> ()) (fun _ -> loc_none) spec
+    (fun j oj -> uint_to_bytes_le oj i.(j));
+  assert_norm (BS.uints_to_bytes_le (as_seq h0 i) ==
+               norm [delta] BS.uints_to_bytes_le (as_seq h0 i))
 
-inline_for_extraction
 let uints_to_bytes_be #t #l len o i =
   let h0 = ST.get () in
-  let inv (h1:mem) (j:nat) = live h1 i /\ live h1 o in
-  let f' (j:size_t{0 <= v j /\ v j < v len}) : Stack unit
-    (requires (fun h -> inv h (v j)))
-    (ensures  (fun h1 _ h2 -> inv h2 (v j + 1))) =
-      let u_i = i.(j) in
-      let b_i = sub o (mul_mod j (size (numbytes t))) (size (numbytes t)) in
-      uint_to_bytes_be b_i u_i in
-  admit();
-  Lib.Loops.for 0ul len inv f'
-*)
+  let a_spec i = unit in
+  let spec (h:mem) = BS.uints_to_bytes_be_inner (as_seq h i) in
+  fill_blocks h0 (size (numbytes t)) len o a_spec (fun _ _ -> ()) (fun _ -> loc_none) spec
+    (fun j oj -> uint_to_bytes_be oj i.(j));
+  assert_norm (BS.uints_to_bytes_be (as_seq h0 i) ==
+               norm [delta] BS.uints_to_bytes_be (as_seq h0 i))
