lib/Lib.ByteBuffer.fsti
@@ -7,7 +7,6 @@ open FStar.Mul
 open LowStar.Buffer
 
 open Lib.IntTypes
-open Lib.RawIntTypes
 open Lib.Buffer
 
 module B = LowStar.Buffer
@@ -28,12 +27,30 @@ val uint_from_be: #t:inttype{~(U128? t)} -> #l:secrecy_level -> uint_t t l -> ui
 inline_for_extraction
 val uint_from_le: #t:inttype{~(U128? t)} -> #l:secrecy_level -> uint_t t l -> uint_t t l
 
-(** Compares two buffers of secret bytes of equal length in constant-time, 
+(** Constructs the equality mask for two buffers of secret integers in constant-time *)
+inline_for_extraction noextract
+val eq_mask:
+    #t:inttype{~(U1? t)}
+  -> #len1:size_t
+  -> #len2:size_t
+  -> b1:lbuffer (uint_t t SEC) len1
+  -> b2:lbuffer (uint_t t SEC) len2
+  -> len:size_t{v len <= v len1 /\ v len <= v len2}
+  -> res:lbuffer (uint_t t SEC) (size 1) ->
+  Stack (uint_t t SEC)
+    (requires fun h ->
+      live h b1 /\ live h b2 /\ live h res /\ disjoint res b1 /\ disjoint res b2 /\
+      v (bget h res 0) == v (ones t SEC))
+    (ensures fun h0 z h1 ->
+      modifies1 res h0 h1 /\
+      v z == v (BS.eq_mask (as_seq h0 b1) (as_seq h0 b2) (v len)))
+
+(** Compares two buffers of secret bytes of equal length in constant-time,
     declassifying the result *)
 inline_for_extraction
 val lbytes_eq: #len:size_t -> b1:lbuffer uint8 len -> b2:lbuffer uint8 len -> Stack bool
   (requires fun h -> live h b1 /\ live h b2)
-  (ensures  fun h0 r h1 -> modifies0 h0 h1 /\ r <==> (as_seq h0 b1 == as_seq h0 b2))
+  (ensures  fun h0 r h1 -> modifies0 h0 h1 /\ r == BS.lbytes_eq (as_seq h0 b1) (as_seq h0 b2))
 
 inline_for_extraction
 val uint_from_bytes_le:
@@ -89,7 +106,7 @@ val uints_from_bytes_le:
   -> o:lbuffer (uint_t t l) len
   -> i:lbuffer (uint_t U8 l) (len *! size (numbytes t)) ->
   Stack unit
-        (requires fun h0 -> live h0 o /\ live h0 i)
+        (requires fun h0 -> live h0 o /\ live h0 i /\ disjoint o i)
         (ensures  fun h0 _ h1 ->
           modifies1 o h0 h1 /\
           as_seq h1 o == BS.uints_from_bytes_le #t #l #(v len) (as_seq h0 i))
@@ -102,7 +119,7 @@ val uints_from_bytes_be:
   -> o:lbuffer (uint_t t l) len
   -> i:lbuffer (uint_t U8 l) (len *! size (numbytes t)) ->
   Stack unit
-        (requires fun h0 -> live h0 o /\ live h0 i)
+        (requires fun h0 -> live h0 o /\ live h0 i /\ disjoint o i)
         (ensures  fun h0 _ h1 ->
           modifies1 o h0 h1 /\
           as_seq h1 o == BS.uints_from_bytes_be #t #l #(v len) (as_seq h0 i))
@@ -115,7 +132,7 @@ val uints_to_bytes_le:
   -> o:lbuffer (uint_t U8 l) (len *! size (numbytes t))
   -> i:lbuffer (uint_t t l) len ->
   Stack unit
-        (requires fun h0 -> live h0 o /\ live h0 i)
+        (requires fun h0 -> live h0 o /\ live h0 i /\ disjoint o i)
         (ensures  fun h0 _ h1 ->
           modifies1 o h0 h1 /\
           as_seq h1 o == BS.uints_to_bytes_le #t #l #(v len) (as_seq h0 i))
